src/coq/TopLevelRefinements.v
@@ -104,7 +104,7 @@ Qed.
 
 Global Instance interp_state_proper {T E F S}
          (h: forall T : Type, E T -> Monads.stateT S (itree F) T)
-  : Proper (eutt Logic.eq ==> Monad.eqm) (State.interp_state h (T := T)).
+  : Proper (eutt Logic.eq ==> Monad.eq1) (State.interp_state h (T := T)).
 Proof.
   einit. ecofix CIH. intros.
 
